Let $G,+$ be a countable abelian group.
Since $G$ is countable, we can write $G = \{0, g_1, g_2, g_3, \dots\}$.
Consider the sequence of sets $$F_n = \left\{\sum_{i = 1}^n a_i g_i \mid -n \le a_i \le n\right\}.$$ 
Fix $g \in G$. Take any $n > j$.
Let $$H_n = \left\{\sum_{\substack{i = 1 \\ g_i \ne g}}^n a_i g_i \mid -n \le a_i \le n\right\}.$$
Notice that $\bigcup_{k = -n}^{n} (kg+H_n) = F_n$.
Define the finite sequence of sets $(B_m^{(n)})_m$ for $m \in \{-n, \dots, n+1\}$ such that  
$B_m^{(n)} = (mg+H_n) \setminus \bigcup_{k=-n}^{m-1}(kg+H_n)$.
It is clear that the elements of $(B_m^{(n)})_m$ are pairwise disjoint and that  \[
    \bigcup_{k = -n}^n B_k^{(n)} = F_n 
.\] 
It follows that $\sum_{k=-n}^{n} \card*{B_k^{(n)}} = \card{F_n}$. We know that 
\begin{align*}
    \card{(g+F_n) \triangle F_n} &= 2 \card{(g + F_n) \setminus F_n} \\
    &= 2 \card{\bigcup_{k = -n}^n ((k+1)g+H_n) \setminus \bigcup_{k = -n}^n (kg+H_n)}\\
    &=  2 \card{((n+1)g+H_n) \setminus \bigcup_{k = -n}^n (kg+H_n)}\\
    &= 2 \card{B_{n+1}^{(n)}}
\end{align*}
So to show that the $F_n$ adheres to the FÃ¸lner criterion, it is sufficient to show that $\frac{\card{B_{n+1}^{(n)}}}{\card{F_n}} \to 0$ as $n \to \infty$.

We claim that $(\card*{B_m^{(n)}})_m$ is a non-increasing sequence. The following calculation shows this.
\begin{align*}
    \card*{B_m^{(n)}} &= \card{(mg+H_n) \setminus \bigcup_{k=-n}^{m-1} kg+H_n}\\
    &= \card{((m-1)g+H_n) \setminus \bigcup_{k=-n}^{m-1}(k-1)g+H_n}\\
    %&= \card{((m-1)g+H_n) \setminus \bigcup_{k=-n-1}^{m-2} kg+H_n}\\
    &\le \card{((m-1)g+H_n) \setminus \bigcup_{k=-n}^{m-2} (k-1)g+H_n} = \card*{B_{m-1}^{(n)}}
\end{align*}
So $\card{F_n} = \sum_{i=-n}^{n} \card{B_i^{(n)}} \le (2n+1) \card*{B_{n+1}^{(n)}}$, which means that $$\frac{\card{B_{n+1}^{(n)}}}{\card{F_n}} \le \frac{1}{2n+1}.$$
So we find that $\lim_{n \to \infty}\frac{\card*{B_{n+1}^{(n)}}}{\card{F_n}} = 0$ which concludes the proof. 
